multi asciiに併せて、等値性の定義を変更した refs: 018

msgpack/MultiAscii.v
@@ -27,8 +27,32 @@ Fixpoint drop (n :nat) (p : positive) :=
       end
   end.
 
+Fixpoint pow (m n : nat) :=
+  match n with
+    | 0 =>
+      1
+    | (S n') =>
+      m * pow m n'
+  end.
+
+Definition nat_of_ascii8 :=
+  nat_of_ascii.
+
 Definition ascii8_of_nat :=
   ascii_of_nat.
+
+Lemma soundness_ascii8 : forall c,
+  ascii8_of_nat (nat_of_ascii8 c) = c.
+Proof.
+apply ascii_nat_embedding.
+Qed.
+
+Definition nat_of_ascii16 bytes :=
+  match bytes with
+    (c1, c2) =>
+    nat_of_ascii c1 * pow 2 8
+    + nat_of_ascii c2
+  end.
 
 Definition ascii16_of_nat n :=
   match n with
@@ -37,6 +61,15 @@ Definition ascii16_of_nat n :=
       let p := P_of_succ_nat n in
         (to_ascii (drop 8 p),
           ascii_of_pos p)
+  end.
+
+Definition nat_of_ascii32 bytes :=
+  match bytes with
+    (c1, c2, c3, c4) =>
+    nat_of_ascii c1   * pow 2 24
+    + nat_of_ascii c2 * pow 2 16
+    + nat_of_ascii c3 * pow 2 8
+    + nat_of_ascii c4
   end.
 
 Definition ascii32_of_nat n :=
@@ -48,6 +81,19 @@ Definition ascii32_of_nat n :=
           to_ascii (drop 16 p),
           to_ascii (drop 8 p),
           ascii_of_pos p)
+  end.
+
+Definition nat_of_ascii64 bytes :=
+  match bytes with
+    (c1, c2, c3, c4, c5, c6, c7, c8) =>
+    nat_of_ascii   c1 * pow 2 56
+    + nat_of_ascii c2 * pow 2 48
+    + nat_of_ascii c3 * pow 2 40
+    + nat_of_ascii c4 * pow 2 32
+    + nat_of_ascii c5 * pow 2 24
+    + nat_of_ascii c6 * pow 2 16
+    + nat_of_ascii c7 * pow 2 8
+    + nat_of_ascii c8
   end.
 
 Definition ascii64_of_nat n :=
